veric/semax_prog.v
@@ -1,6 +1,7 @@
 Require Import VST.veric.juicy_base.
 Require Import VST.veric.juicy_mem (*VST.veric.juicy_mem_lemmas VST.veric.juicy_mem_ops*).
 Require Import VST.veric.res_predicates.
+Require Import VST.veric.external_state.
 Require Import VST.veric.extend_tc.
 Require Import VST.veric.Clight_seplog.
 Require Import VST.veric.Clight_assert_lemmas.
@@ -24,9 +25,13 @@ Require Import Coq.Logic.JMeq.
 
 Import Ctypes Clight.
 
-Lemma funspec_eq {sig cc A P Q P' Q' Pne Qne Pne' Qne'}:
+Section mpred.
+
+Context `{!heapGS Σ}.
+
+Lemma funspec_eq {sig cc A P Q P' Q'}:
       P = P' -> Q=Q' ->
-      mk_funspec sig cc A P Q Pne Qne = mk_funspec sig cc A P' Q' Pne' Qne'.
+      mk_funspec sig cc A P Q = mk_funspec sig cc A P' Q'.
 Proof. intros. subst. f_equal; apply proof_irr. Qed.
 
 Fixpoint match_globvars (gvs: list (ident * globvar type)) (V: varspecs) : bool :=
@@ -57,25 +62,25 @@ destruct H0 as [? [? ?]].
 intros id t ?.
 unfold make_tycontext, temp_types in H4.
 unfold make_tycontext_t in H4.
-set (f1 := fun param : ident * type => PTree.set (fst param) (snd param)) in *.
-set (f2 := fun (temp : ident * type) (tenv : PTree.tree type) =>
-            let (id, ty) := temp in PTree.set id ty tenv) in *.
+set (f1 := fun param : ident * type => Maps.PTree.set (fst param) (snd param)) in *.
+set (f2 := fun (temp : ident * type) (tenv : Maps.PTree.tree type) =>
+            let (id, ty) := temp in Maps.PTree.set id ty tenv) in *.
 unfold Map.get, make_tenv.
 (***)
-set (t0 := PTree.empty type) in *.
-set (v0 := PTree.empty val) in *.
-assert (t0 ! id = Some t ->
-   exists v : val, v0 ! id = Some v /\ tc_val' t v). {
+set (t0 := Maps.PTree.empty type) in *.
+set (v0 := Maps.PTree.empty val) in *.
+assert (Maps.PTree.get id t0 = Some t ->
+   exists v : val, Maps.PTree.get id v0 = Some v /\ tc_val' t v). {
   subst t0 v0.
-  intros. rewrite PTree.gempty in H5; inv H5.
+  intros. rewrite Maps.PTree.gempty in H5; inv H5.
 }
 set (t1 := fold_right f2 t0 temps) in *.
 set (v1 := create_undef_temps temps) in *.
 unfold create_undef_temps in v1.
 fold v0 in v1.
 clearbody t0. clearbody v0.
-assert (t1 ! id = Some t ->
-   exists v : val, v1 ! id = Some v /\ tc_val' t v). {
+assert (Maps.PTree.get id t1 = Some t ->
+   exists v : val, Maps.PTree.get id v1 = Some v /\ tc_val' t v). {
   subst t1 v1.
   clear - H5.
   revert t0 v0 H5.
@@ -83,11 +88,11 @@ assert (t1 ! id = Some t ->
   destruct (H5 H) as [v [? ?]].
   eauto.
   destruct (ident_eq i id). subst.
-  rewrite PTree.gss. eexists; split; eauto.
+  rewrite Maps.PTree.gss. eexists; split; eauto.
   intro Hx; contradiction Hx; auto.
-  rewrite PTree.gso by auto.
+  rewrite -> Maps.PTree.gso by auto.
   eapply IHtemps; eauto.
-  rewrite PTree.gso in H; auto.
+  rewrite Maps.PTree.gso in H; auto.
 }
 clearbody v1. clearbody t1.
 clear H5 t0 v0.
@@ -99,15 +104,15 @@ inv H1.
 auto.
 unfold f1 in H4. simpl in H4.
 destruct (ident_eq i id).
-subst i. rewrite PTree.gss in H4.
+subst i. setoid_rewrite Maps.PTree.gss in H4.
 inv H4.
 exists v.
 destruct H.
 split; [| intro; auto].
 inv H0.
-assert ((PTree.set id v v1) ! id = Some v).
-apply PTree.gss.
-forget (PTree.set id v v1) as e1.
+assert (Maps.PTree.get id (Maps.PTree.set id v v1) = Some v).
+apply Maps.PTree.gss.
+forget (Maps.PTree.set id v v1) as e1.
 clear - H H5 H2 H0 H1.
 revert e1 H args H0 H1 H2; induction params as [|[??]]; destruct args; simpl; intros; try contradiction.
 inv H1. auto.
@@ -116,13 +121,13 @@ simpl in H5.
 apply Decidable.not_or in H5.
 destruct H5.
 eapply IHparams; try apply H1; auto.
-rewrite PTree.gso by auto; auto.
+rewrite -> Maps.PTree.gso by auto; auto.
 destruct H.
-rewrite PTree.gso in H4 by auto.
+setoid_rewrite -> Maps.PTree.gso in H4; auto.
 inv H0.
 eapply IHparams; try apply H1; auto.
 eassumption.
-rewrite PTree.gso; auto.
+rewrite Maps.PTree.gso; auto.
 Qed.
 
 Lemma typecheck_var_environ_i:
@@ -136,25 +141,25 @@ Proof.
 intros.
 hnf; intros.
 unfold make_tycontext_v, make_venv, Map.get.
-set (f := fun (var : ident * type) (venv : PTree.tree type) =>
-    let (id0, ty0) := var in PTree.set id0 ty0 venv).
-transitivity (option_map snd (ve' ! id) = Some ty).
-2:{ destruct (ve' ! id) as [[??]|]; simpl; split; intro.
+set (f := fun (var : ident * type) (venv : Maps.PTree.tree type) =>
+    let (id0, ty0) := var in Maps.PTree.set id0 ty0 venv).
+transitivity (option_map snd (Maps.PTree.get id ve') = Some ty).
+2:{ destruct (Maps.PTree.get id ve') as [[??]|]; simpl; split; intro.
      inv H1; exists b; eauto. destruct H1; inv H1; auto.
      inv H1. destruct H1; inv H1.
 }
-assert ((fold_right f (PTree.empty type) vars) ! id =
-           option_map snd (ve' ! id)).
+assert ((fold_right f (Maps.PTree.empty type) vars) !! id =
+           option_map snd (ve' !! id)).
 2: rewrite H1; split; auto.
-set (s := PTree.empty type).
+set (s := Maps.PTree.empty type).
 set (r := empty_env) in *.
-assert (s ! id = option_map snd (r ! id)).
+assert (s !! id = option_map snd (r !! id)).
 subst s r.
 unfold empty_env.
-rewrite !PTree.gempty.
+setoid_rewrite (Maps.PTree.gempty _ id).
 reflexivity.
-assert (In id (map fst vars) -> s ! id = None)
-   by (intros; apply PTree.gempty).
+assert (In id (map fst vars) -> s !! id = None)
+   by (intros; apply Maps.PTree.gempty).
 clearbody r.
 clearbody s.
 induction H0.
@@ -163,24 +168,24 @@ inv H.
 destruct (ident_eq id0 id); simpl in *.
 subst.
 spec H2; auto.
-rewrite H2 in *.
-rewrite PTree.gss in *.
+rewrite -> H2 in *.
+setoid_rewrite -> Maps.PTree.gss.
 clear - H3 H6.
-set (e1 := PTree.set id (b1, ty0) e) in *.
-transitivity (option_map snd e1 ! id).
-subst e1. rewrite PTree.gss; reflexivity.
+set (e1 := Maps.PTree.set id (b1, ty0) e) in *.
+transitivity (option_map snd (e1 !! id)).
+subst e1. setoid_rewrite Maps.PTree.gss; reflexivity.
 induction H3. auto.
 simpl in H6.
 apply Decidable.not_or in H6.
 destruct H6.
-rewrite PTree.gso in * by auto.
-auto.
-rewrite PTree.gso in * by auto.
+setoid_rewrite Maps.PTree.gso in IHalloc_variables; auto.
+setoid_rewrite Maps.PTree.gso; auto.
 apply IHalloc_variables; auto.
+setoid_rewrite Maps.PTree.gso; auto.
 Qed.
 
 Section semax_prog.
-Context (Espec: OracleKind).
+Context (Espec : OracleKind) `{!externalGS OK_ty Σ}.
 
 Definition prog_contains (ge: genv) (fdecs : list (ident * Clight.fundef)) : Prop :=
      forall id f, In (id,f) fdecs ->
@@ -188,7 +193,7 @@ Definition prog_contains (ge: genv) (fdecs : list (ident * Clight.fundef)) : Pro
 
 Definition entry_tempenv (te: temp_env) (f: function) (vl: list val) :=
    length vl = length f.(fn_params) /\
-   forall id v, PTree.get id te = Some v ->
+   forall id v, Maps.PTree.get id te = Some v ->
                       In (id,v)
                        (combine (map (@fst _ _) f.(fn_params)) vl
                           ++ map (fun tv => (fst tv, Vundef)) f.(fn_temps)).
@@ -199,15 +204,15 @@ andb
     (compute_list_norepet (map (@fst _ _) (fn_vars f))).
 
 Definition semax_body
-   (V: varspecs) (G: funspecs) {C: compspecs} (f: function) (spec: ident * funspec): Prop :=
-match spec with (_, mk_funspec fsig cc A P Q _ _) =>
+   (V: varspecs) (G: funspecs) {C: compspecs} E (f: function) (spec: ident * funspec): Prop :=
+match spec with (_, mk_funspec fsig cc A P Q) =>
   fst fsig = map snd (fst (fn_funsig f)) /\
   snd fsig = snd (fn_funsig f) /\
-forall Espec ts (x:dependent_type_functor_rec ts A mpred),
-  semax Espec (func_tycontext f V G nil)
-      (fun rho => close_precondition (map fst f.(fn_params)) (P ts x) rho * stackframe_of f rho)
+forall Espec `(externalGS OK_ty Σ) (x:A),
+  semax Espec E (func_tycontext f V G nil)
+      (fun rho => close_precondition (map fst f.(fn_params)) (P x) rho ∗ stackframe_of f rho)
        f.(fn_body)
-      (frame_ret_assert (function_body_ret_assert (fn_return f) (Q ts x)) (stackframe_of f))
+      (frame_ret_assert (function_body_ret_assert (fn_return f) (Q x)) (stackframe_of f))
 end.
 
 Definition genv_contains (ge: Genv.t Clight.fundef type) (fdecs : list (ident * Clight.fundef)) : Prop :=
@@ -218,16 +223,16 @@ Lemma genv_prog_contains (ge:genv) fdecs: prog_contains ge fdecs = genv_contains
 Proof. reflexivity. Qed.
 
 Definition semax_func (V: varspecs) (G: funspecs) {C: compspecs} (ge: Genv.t Clight.fundef type)
-       (fdecs: list (ident * Clight.fundef)) (G1: funspecs) : Prop :=
+       E (fdecs: list (ident * Clight.fundef)) (G1: funspecs) : Prop :=
 match_fdecs fdecs G1 /\ genv_contains ge fdecs /\
 forall (ge': Genv.t Clight.fundef type) (Gfs: forall i,  sub_option (Genv.find_symbol ge i) (Genv.find_symbol ge' i))
-         (Gffp: forall b, sub_option (Genv.find_funct_ptr ge b) (Genv.find_funct_ptr ge' b))
-n, believe Espec (nofunc_tycontext V G) (Build_genv ge' (@cenv_cs C)) (nofunc_tycontext V G1) n.
+         (Gffp: forall b, sub_option (Genv.find_funct_ptr ge b) (Genv.find_funct_ptr ge' b)),
+  ⊢ believe Espec E (nofunc_tycontext V G) (Build_genv ge' (@cenv_cs C)) (nofunc_tycontext V G1).
 
 Lemma semax_func_cenv_sub CS CS' (CSUB: cenv_sub (@cenv_cs CS) (@cenv_cs CS')) ge ge'
   (Gfs: forall i,  sub_option (Genv.find_symbol ge i) (Genv.find_symbol ge' i))
   (Gffp: forall b, sub_option (Genv.find_funct_ptr ge b) (Genv.find_funct_ptr ge' b))
-  V G fdecs G1 (H: @semax_func  V G CS ge fdecs G1): @semax_func  V G CS' ge' fdecs G1.
+  V G E fdecs G1 (H: semax_func V G (C := CS) ge E fdecs G1): semax_func V G (C := CS') ge' E fdecs G1.
 Proof.
 destruct H as [MF [GC B]]; split; [trivial | split].
 + hnf; intros. destruct (GC _ _ H) as [b [Hb1 Hb2]]. exists b; split.
@@ -238,38 +243,39 @@ assert (Q1: forall i, sub_option (Genv.find_symbol ge i) (Genv.find_symbol ge2 i
 { intros. eapply sub_option_trans. apply Gfs. apply Gfs0. }
 assert (Q2: forall b, sub_option (Genv.find_funct_ptr ge b) (Genv.find_funct_ptr ge2 b)).
 { intros. eapply sub_option_trans. apply Gffp. apply Gffp0. }
-apply (@believe_cenv_sub_L CS Espec CS' {| genv_genv := ge2; genv_cenv := cenv_cs |} (nofunc_tycontext V G) (nofunc_tycontext V G)).
-intros; apply tycontext_sub_refl. apply CSUB. apply (B _ Q1 Q2 n).
+rewrite - (believe_cenv_sub_L(CS := CS) Espec (CS' := CS') {| genv_genv := ge2; genv_cenv := cenv_cs |} E (nofunc_tycontext V G) (nofunc_tycontext V G)); eauto.
+intros; apply tycontext_sub_refl.
 Qed.
 Lemma semax_func_mono CS CS' (CSUB: cspecs_sub CS CS') ge ge'
   (Gfs: forall i,  sub_option (Genv.find_symbol ge i) (Genv.find_symbol ge' i))
   (Gffp: forall b, sub_option (Genv.find_funct_ptr ge b) (Genv.find_funct_ptr ge' b))
-  V G fdecs G1 (H: @semax_func  V G CS ge fdecs G1): @semax_func  V G CS' ge' fdecs G1.
+  V G E fdecs G1 (H: semax_func(C := CS) V G ge E fdecs G1): semax_func(C := CS') V G ge' E fdecs G1.
 Proof.
   destruct CSUB as [CSUB _].
-  eapply (@semax_func_cenv_sub _ _ CSUB); eassumption.
+  eapply (semax_func_cenv_sub _ _ CSUB); eassumption.
 Qed.
 
-Definition main_pre {Z} (prog: program) (ora: Z) : (ident->val) -> argsassert :=
-(fun gv gvals => !!(gv = genviron2globals (fst gvals) /\ snd gvals=nil)
-       && globvars2pred gv (prog_vars prog) * has_ext ora).
+Definition main_pre (prog: program) (ora: OK_ty) : (ident->val) -> argsEnviron -> mpred :=
+(fun gv gvals => ⌜gv = genviron2globals (fst gvals) /\ snd gvals=nil⌝
+       ∧ globvars2pred gv (prog_vars prog) ∗ has_ext ora).
 
-Lemma main_pre_vals_nil {Z prog ora gv g vals}:
-      @main_pre Z prog ora gv (g, vals) |-- !!(vals=nil).
-Proof. unfold main_pre; simpl. intros ? [? [? [? [[X ?] _]]]]. apply X.
+Lemma main_pre_vals_nil {prog ora gv g vals}:
+      main_pre prog ora gv (g, vals) ⊢ ⌜vals=nil⌝.
+Proof.
+  unfold main_pre; simpl. by iIntros "((_ & ->) & _)".
 Qed.
 
 Definition Tint32s := Tint I32 Signed noattr.
 
-Definition main_post (prog: program) : (ident->val) -> assert :=
-(fun _ _ => TT).
+Definition main_post (prog: program) : (ident->val) -> environ -> mpred :=
+(fun _ _ => True).
 
-Definition main_spec_ext' {Z} (prog: program) (ora: Z)
-(post: (ident->val) -> environ ->pred rmap): funspec :=
-NDmk_funspec (nil, tint) cc_default (ident->val) (main_pre prog ora) post.
+Definition main_spec_ext' (prog: program) (ora: OK_ty)
+(post: (ident->val) -> environ -> mpred): funspec :=
+mk_funspec (nil, tint) cc_default (ident->val) (main_pre prog ora) post.
 
 Definition main_spec_ext (prog: program) (ora: OK_ty): funspec :=
-NDmk_funspec (nil, tint) cc_default (ident->val) (main_pre prog ora) (main_post prog).
+mk_funspec (nil, tint) cc_default (ident->val) (main_pre prog ora) (main_post prog).
 
 Definition is_Internal (prog : program) (f : ident) :=
 match Genv.find_symbol (Genv.globalenv prog) f with
@@ -289,15 +295,15 @@ Definition postcondition_allows_exit retty :=
    forall
       v  ora (jm : juicy_mem),
       tc_option_val retty v ->
-      ext_compat ora (m_phi jm) ->
+(*      ext_compat ora (m_phi jm) -> *)
       ext_spec_exit OK_spec v ora jm.
 
 Definition semax_prog {C: compspecs}
        (prog: program) (ora: OK_ty) (V: varspecs) (G: funspecs) : Prop :=
 compute_list_norepet (prog_defs_names prog) = true  /\
 all_initializers_aligned prog /\
-PTree.elements cenv_cs = PTree.elements (prog_comp_env prog) /\
-@semax_func V G C (Genv.globalenv prog) (prog_funct prog) G /\
+Maps.PTree.elements cenv_cs = Maps.PTree.elements (prog_comp_env prog) /\
+@semax_func V G C (Genv.globalenv prog) ⊤ (prog_funct prog) G /\
 match_globvars (prog_vars prog) V = true /\
 match find_id prog.(prog_main) G with
 | Some s => exists post,
@@ -307,123 +313,44 @@ end.
 
 Lemma semax_func_nil:
 forall
- V G {C: compspecs} ge, @semax_func V G C ge nil nil.
+ V G {C: compspecs} ge E, semax_func(C := C) V G ge E nil nil.
 Proof.
 intros; split. constructor. split; [ hnf; intros; inv H | intros].
-intros b fsig cc ty P Q ? w ? Hext ?.
-hnf in H0.
-destruct H0 as [b' [NEP [NEQ [? ?]]]].
-simpl in H0.
-rewrite PTree.gempty in H0. inv H0.
-Qed.
-
-Program Definition HO_pred_eq {T}{agT: ageable T}{EO: Ext_ord T}
-(A: Type) (P: A -> pred T) (A': Type) (P': A' -> pred T) : pred nat :=
-fun v => exists H: A=A',
- match H in (_ = A) return (A -> pred T) -> Prop with
- | refl_equal => fun (u3: A -> pred T) =>
-                                forall x: A, (P x <=> u3 x) v
- end P'.
-Next Obligation.
-split; repeat intro.
-destruct H0. exists x.
-destruct x.
-intros. specialize (H0 x). eapply pred_hereditary; eauto.
-
-destruct H0. exists x.
-destruct x.
-intros. specialize (H0 x). eapply pred_upclosed; eauto.
-Qed.
-
-Lemma laterR_level: forall w w' : rmap, laterR w w' -> (level w > level w')%nat.
-Proof.
-induction 1.
-unfold age in H. rewrite <- ageN1 in H.
-change rmap with R.rmap; change ag_rmap with R.ag_rmap.
-rewrite (ageN_level _ _ _ H). generalize (@level _ R.ag_rmap y). intros; lia.
-lia.
-Qed.
-
-Lemma necR_level:  forall w w' : rmap, necR w w' -> (level w >= level w')%nat.
-Proof.
-induction 1.
-unfold age in H. rewrite <- ageN1 in H.
-change rmap with R.rmap; change ag_rmap with R.ag_rmap.
-rewrite (ageN_level _ _ _ H). generalize (@level _ R.ag_rmap y). intros; lia.
-lia.
-lia.
-Qed.
-
-Lemma HO_pred_eq_i1:
-forall A P P' m,
-  approx (level m) oo  P = approx (level m) oo P' ->
-(|> HO_pred_eq A P A  P') m.
-Proof.
-intros.
-unfold HO_pred_eq.
-intros ?m ?.
-hnf.
-exists (refl_equal A).
-intros.
-generalize (f_equal (fun f => f x) H); clear H; intro.
-simpl in H0.
-unfold compose in *.
-apply clos_trans_t1n in H0.
-revert H; induction H0; intros.
-2 : { apply IHclos_trans_1n.
-  unfold age,age1 in H. unfold ag_nat in H. unfold natAge1 in H. destruct x0; inv H.
-  clear - H1.
-  assert (forall w, app_pred (approx (level (S y)) (P x)) w <-> app_pred (approx (level (S y)) (P' x)) w).
-  { intros; rewrite H1; tauto. }
-  apply pred_ext; intros w ?; destruct (H w); simpl in *; intuition.
-  apply H0; auto. clear - H4.  unfold natLevel in *. lia.
-  apply H2; auto. clear - H4.  unfold natLevel in *. lia. }
-unfold age,age1 in H. unfold ag_nat in H. unfold natAge1 in H. destruct x0; inv H.
-intros z ?.
-split; intros ? a' ? Hext%ext_level ?.
-assert (app_pred (approx (level (S y)) (P x)) a').
-{ simpl. split; auto. unfold natLevel.  apply necR_level in H1.
-  lia. }
-rewrite H0 in H3.
-simpl in H3. destruct H3; auto.
-assert (app_pred (approx (level (S y)) (P' x)) a').
-{ simpl. split; auto. unfold natLevel.  apply necR_level in H1.
-  lia. }
-rewrite <- H0 in H3.
-simpl in H3. destruct H3; auto.
+iIntros (?????? Hclaims).
+destruct Hclaims as (? & Hlookup & ?).
+setoid_rewrite Maps.PTree.gempty in Hlookup. discriminate.
 Qed.
 
 Lemma semax_func_cons_aux:
-forall (psi: genv) id fsig1 cc1 A1 P1 Q1 NEP1 NEQ1 fsig2 cc2 A2 P2 Q2 (V: varspecs) (G': funspecs) {C: compspecs} b fs,
+forall (psi: genv) id fsig1 cc1 A1 P1 Q1 fsig2 cc2 A2 P2 Q2 (V: varspecs) (G': funspecs) {C: compspecs} b fs,
 Genv.find_symbol psi id = Some b ->
 ~ In id (map (fst (A:=ident) (B:=Clight.fundef)) fs) ->
 match_fdecs fs G'  ->
-claims  psi (nofunc_tycontext V ((id, mk_funspec fsig1 cc1 A1 P1 Q1 NEP1 NEQ1) :: G')) (Vptr b Ptrofs.zero) fsig2 cc2 A2 P2 Q2 ->
+claims  psi (nofunc_tycontext V ((id, mk_funspec fsig1 cc1 A1 P1 Q1) :: G')) (Vptr b Ptrofs.zero) fsig2 cc2 A2 P2 Q2 ->
 fsig1=fsig2 /\ cc1 = cc2 /\ A1=A2 /\ JMeq P1 P2 /\ JMeq Q1 Q2.
 Proof.
 intros until fs. intros H Hin Hmf; intros.
-destruct H0 as [id' [NEP2 [NEQ2 [? ?]]]].
+destruct H0 as [id' [? ?]].
 simpl in H0.
 destruct (eq_dec id id').
-subst id'. rewrite PTree.gss in H0. inv H0.
+subst id'. setoid_rewrite Maps.PTree.gss in H0. inv H0.
 apply inj_pair2 in H6. apply inj_pair2 in H7.
-subst.
-split; auto.
-rewrite PTree.gso in H0 by auto.
+subst; auto.
+setoid_rewrite Maps.PTree.gso in H0; last done.
 exfalso.
 destruct H1 as [b' [? ?]].
 symmetry in H2; inv H2.
 assert (In id' (map (@fst _ _) G')).
 clear - H0.
 revert H0; induction G'; simpl; intros; auto.
-rewrite PTree.gempty in H0; inv H0.
+rewrite Maps.PTree.gempty in H0; inv H0.
 destruct (eq_dec id' (fst a)). subst.
 destruct a; simpl in *.
-rewrite PTree.gss in H0 by auto. inv  H0.
+rewrite -> Maps.PTree.gss in H0 by auto. inv  H0.
 auto.
 destruct a; simpl in *.
-destruct (eq_dec i id'). subst. rewrite PTree.gss in H0. auto.
-rewrite PTree.gso in H0 by auto.
+destruct (eq_dec i id'). subst. rewrite Maps.PTree.gss in H0. auto.
+rewrite -> Maps.PTree.gso in H0 by auto.
 right; apply IHG'; auto.
 destruct (eq_dec id id').
 2: apply (Genv.global_addresses_distinct psi n H H1); auto.
@@ -447,12 +374,12 @@ Proof.
 extensionality rho.
 unfold stackframe_of'. forget (fn_vars f) as vars.
 induction vars; simpl; trivial.
-inv COMPLETE. rewrite (var_block'_cenv_sub CSUB _ _ H1), IHvars; clear IHvars; trivial.
+inv COMPLETE. rewrite (var_block'_cenv_sub CSUB _ _ H1) IHvars; clear IHvars; trivial.
 Qed.
 
 Lemma var_block_cspecs_sub {CS CS'} (CSUB: cspecs_sub CS CS') sh a
 (CT: complete_type (@cenv_cs CS) (@snd ident type a) = true):
-@var_block sh CS a = @var_block sh CS' a.
+var_block(cs := CS) sh a = var_block(cs := CS') sh a.
 Proof.
 extensionality rho. destruct CSUB as [CSUB _].
 unfold var_block. unfold expr.sizeof. rewrite (cenv_sub_sizeof CSUB); trivial.
@@ -460,37 +387,37 @@ Qed.
 
 Lemma stackframe_of_cspecs_sub {CS CS'} (CSUB: cspecs_sub CS CS') f
   (COMPLETE : Forall (fun it : ident * type => complete_type (@cenv_cs CS) (snd it) = true) (fn_vars f)):
-@stackframe_of CS f = @stackframe_of CS' f .
+stackframe_of(cs := CS) f = stackframe_of(cs := CS') f .
 Proof.
 extensionality rho.
 unfold stackframe_of. forget (fn_vars f) as vars.
 induction vars; simpl; trivial.
-inv COMPLETE. rewrite (var_block_cspecs_sub CSUB _ _ H1), IHvars; clear IHvars; trivial.
+inv COMPLETE. rewrite (var_block_cspecs_sub CSUB _ _ H1) IHvars; clear IHvars; trivial.
 Qed.
 
-Lemma semax_body_cenv_sub {CS CS'} (CSUB: cspecs_sub CS CS') V G f spec
+Lemma semax_body_cenv_sub {CS CS'} (CSUB: cspecs_sub CS CS') V G E f spec
 (COMPLETE : Forall (fun it : ident * type => complete_type (@cenv_cs CS) (snd it) = true) (fn_vars f)):
-@semax_body V G CS f spec -> @semax_body V G CS' f spec.
+semax_body(C := CS) V G E f spec -> semax_body(C := CS') V G E f spec.
 Proof.
 destruct spec.
 destruct f0.
 intros [H' [H'' H]]; split3; auto. clear H' H''.
 intros.
-  specialize (H Espec0 ts x).
-rewrite <- (stackframe_of_cspecs_sub CSUB); [apply (semax_cssub CSUB); apply H | trivial].
+  specialize (H Espec0 H0 x).
+rewrite <- (stackframe_of_cspecs_sub CSUB); [apply (semax_cssub _ CSUB); apply H | trivial].
 Qed.
 
-Lemma semax_body_type_of_function {V G cs f i phi} (SB : @semax_body V G cs f (i, phi))
+Lemma semax_body_type_of_function {V G cs E f i phi} (SB : @semax_body V G cs E f (i, phi))
       (CC: fn_callconv f = callingconvention_of_funspec phi):
 type_of_function f = type_of_funspec phi.
 Proof.
-  destruct phi as [[? ?] ? ? ? ? ? ?]. destruct SB as [? [? _]].
+  destruct phi as [[? ?] ? ? ? ?]. destruct SB as [? [? _]].
   unfold type_of_function; simpl in *. subst.
   rewrite <- TTL1; trivial.
 Qed.
 
 Lemma semax_func_cons
-     fs id f fsig cc (A: TypeTree) P Q NEP NEQ (V: varspecs) (G G': funspecs) {C: compspecs} ge b :
+     fs id f fsig cc (A: Type) P Q (V: varspecs) (G G': funspecs) {C: compspecs} ge E b :
   andb (id_in_list id (map (@fst _ _) G))
   (andb (negb (id_in_list id (map (@fst ident Clight.fundef) fs)))
     (semax_body_params_ok f)) = true ->
@@ -502,10 +429,10 @@ Lemma semax_func_cons
    f.(fn_callconv) = cc ->
    Genv.find_symbol ge id = Some b ->
    Genv.find_funct_ptr ge b = Some (Internal f) ->
-  semax_body V G f (id, mk_funspec fsig cc A P Q NEP NEQ) ->
-  semax_func V G ge fs G' ->
-  semax_func V G ge ((id, Internal f)::fs)
-       ((id, mk_funspec fsig cc A P Q NEP NEQ)  :: G').
+  semax_body V G E f (id, mk_funspec fsig cc A P Q) ->
+  semax_func V G ge E fs G' ->
+  semax_func V G ge E ((id, Internal f)::fs)
+       ((id, mk_funspec fsig cc A P Q)  :: G').
 Proof.
 intros H' COMPLETE Hvars Hcc Hb1 Hb2 SB [HfsG' [Hfs HG]].
 apply andb_true_iff in H'.
@@ -518,13 +445,9 @@ split3.
 { apply id_in_list_true in Hin. rewrite negb_true_iff in Hni.
   hnf; intros. destruct H0; [ symmetry in H0; inv H0 | apply (Hfs _ _ H0)].
   exists b; split; trivial. }
-intros ge' H0 HGG n.
+intros ge' H0 HGG.
 specialize (HG _ H0 HGG).
-hnf in HG |- *.
-intros v fsig0 cc' A' P' Q'.
-apply derives_imp.
-clear n.
-intros n ?.
+iIntros (???????).
 subst cc.
 rewrite <- Genv.find_funct_find_funct_ptr in Hb2.
 apply negb_true_iff in Hni.
@@ -532,10 +455,11 @@ apply id_in_list_false in Hni.
 destruct (eq_dec  (Vptr b Ptrofs.zero) v) as [?H|?H].
 * (* Vptr b Ptrofs.zero = v *)
 subst v.
-right.
-exists b; exists f.
-split.
+iRight.
+iExists b; iExists f.
+iSplit.
 +
+iPureIntro.
 apply andb_true_iff in H.
 destruct H as [H H'].
 apply compute_list_norepet_e in H.
@@ -547,62 +471,45 @@ split. { specialize (HGG b). unfold fundef in HGG;  rewrite Hb2 in HGG; simpl in
 split; auto.
 split; auto.
 split; auto.
-destruct H1 as [id' [NEP' [NEQ' [? [b' [FS' Hbb']]]]]].
+destruct H1 as [id' [? [b' [FS' Hbb']]]].
 symmetry in Hbb'; inv Hbb'.
 destruct (eq_dec id id').
- - subst. simpl in H1. rewrite PTree.gss in H1.
-   symmetry in H1; inv H1. apply inj_pair2 in H6. apply inj_pair2 in H7. subst Q' P'. simpl in *.
+ - subst. simpl in H1. setoid_rewrite Maps.PTree.gss in H1.
+   symmetry in H1; inv H1. apply inj_pair2 in H6. apply inj_pair2 in H7. subst Q0 P0. simpl in *.
    destruct SB. apply list_norepet_app in H. tauto.
  - specialize (H0 id); unfold fundef in H0. simpl in H0.  rewrite Hb1 in H0; simpl in H0.
    simpl in FS'.
-   elim (Genv.global_addresses_distinct ge' n0 H0 FS'); trivial.
+   elim (Genv.global_addresses_distinct ge' n H0 FS'); trivial.
 +
-intros Delta' CS' ? k NK EK HDelta' ? w KW EW CSUB.
-intros ts x.
-simpl in H1. specialize (H0 id); unfold fundef in H0; simpl in H0. rewrite Hb1 in H0; simpl in H0.
-pose proof (semax_func_cons_aux (Build_genv ge' cenv_cs) _ _ _ _ _ _ _ _ _ _ _ _ _ _ _ _ _ H0 Hni HfsG' H1).
-destruct H2 as [H4' [H4 [H4a [H4b H4c]]]].
-subst A' fsig0 cc'.
+iIntros (?? HDelta' CSUB ?) "!>".
+specialize (H0 id); unfold fundef in H0; simpl in H0. rewrite Hb1 in H0; simpl in H0.
+pose proof (semax_func_cons_aux (Build_genv ge' cenv_cs) _ _ _ _ _ _ _ _ _ _ _ _ _ _ _ H0 Hni HfsG' H1) as [H4' [H4 [H4a [H4b H4c]]]].
+subst A0 fsig0 cc0.
 apply JMeq_eq in H4b.
 apply JMeq_eq in H4c.
-subst P' Q'.
-destruct SB as [X [Y SB]]. specialize (SB Espec ts x). simpl fst in X. simpl snd in Y.
-specialize (SB k).
-apply now_later.
+subst P0 Q0.
+destruct SB as [X [Y SB]]. specialize (SB Espec externalGS0 x). simpl fst in X. simpl snd in Y.
 rewrite <- (stackframe_of'_cenv_sub CSUB); trivial.
-apply (semax'_cenv_sub CSUB).
-simpl in EK, EW; subst.
-clear - SB NK KW HDelta' X.
-rewrite semax_fold_unfold in SB|-*. intros gx DD CS' ? u WU EU [SUB GX] ? v UV EV BEL.
-simpl in EU, EV; subst.
-assert (HDD: tycontext_sub (func_tycontext f V G nil) DD).
+iApply (semax'_cenv_sub _ CSUB).
+clear - SB HDelta' X.
+rewrite semax_unfold in SB; rewrite semax_fold_unfold. iIntros (? DD ? [SUB GX]) "BEL".
+assert (HDD: tycontext_sub E (func_tycontext f V G nil) DD).
 { unfold func_tycontext, func_tycontext'. simpl.
 eapply tycontext_sub_trans; eauto. }
-assert (WV: @necR nat ag_nat w v). { eapply necR_trans.  apply WU. apply UV. }
-specialize (SB gx DD CS' _ _ KW (eq_refl _) (conj HDD GX) _ _ WV (eq_refl _) BEL).
-revert SB.
-eapply allp_derives; intro kk.
-apply allp_derives; intro F.
-apply allp_derives; intro curf.
-apply imp_derives; auto.
-unfold guard.
-apply allp_derives; intro tx.
-eapply allp_derives; intro vx.
-eapply subp_derives; auto.
-apply andp_derives; auto.
-apply andp_derives; auto.
-apply sepcon_derives; auto.
-apply andp_left1.
-apply sepcon_derives; auto.
-apply andp_left2; trivial.
+iPoseProof (SB with "BEL") as "#SB".
+iIntros (kk F curf) "H"; iPoseProof ("SB" with "H") as "#guard".
+rewrite /guard' /_guard.
+iIntros (??) "!>".
+iIntros "H"; iApply "guard".
+iDestruct "H" as "($ & ($ & (((_ & $) & $) & _)) & $)".
 * (***   Vptr b Ptrofs.zero <> v'  ********)
-eapply (HG n v fsig0 cc' A' P' Q'); auto.
-destruct H1 as [id' [NEP' [NEQ' [? B]]]].
-simpl in H1. rewrite PTree.gsspec in H1.
+iApply HG; iPureIntro.
+destruct H1 as [id' [? B]].
+simpl in H1. setoid_rewrite Maps.PTree.gsspec in H1.
 destruct (peq id' id); subst.
 - specialize (H0 id); unfold fundef in H0; simpl in H0.
   destruct B as [? [? ?]]. rewrite Hb1 in H0; simpl in H0. unfold fundef in H3; simpl in H3; congruence.
-- exists id', NEP', NEQ'; split; auto.
+- exists id'; split; auto.
 Qed.
 
 (* EXPERIMENT
@@ -625,14 +532,11 @@ Qed.
 *)
 
 Lemma semax_external_FF:
-forall Espec ef A n,
-@semax_external Espec ef A (fun _ _ _ => FF) (fun _ _ _ => FF) n.
+forall Espec `{!externalGS OK_ty Σ} E ef A,
+⊢ semax_external Espec E ef A (fun _ _ => False) (fun _ _ => False).
 intros.
-hnf; intros.
-simpl.
-intros.
-destruct H3 as [? [? [? [? [? ?]]]]].
-contradiction.
+iIntros (?????) "!> !>".
+iIntros "(_ & [] & _)".
 Qed.
 
 Lemma TTL6 {l}: typelist_of_type_list (typelist2list l) = l.
@@ -649,7 +553,7 @@ forall (V: varspecs) (G: funspecs) {C: compspecs} ge fs id ef argsig retsig A P 
   (forall gx ts x (ret : option val),
      (Q ts x (make_ext_rval gx (rettype_of_type retsig) ret)
         && !!Builtins0.val_opt_has_rettype ret (rettype_of_type retsig)
-        |-- !!tc_option_val retsig ret)) ->
+        ⊢ !!tc_option_val retsig ret)) ->
   Genv.find_symbol ge id = Some b -> Genv.find_funct_ptr ge b = Some (External ef argsig retsig cc) ->
   (forall n, semax_external Espec ef A P Q n) ->
   semax_func V G ge fs G' ->
@@ -693,10 +597,10 @@ eapply (Hf n v' fsig' cc' A' P' Q'); auto.
 destruct H0 as [id' [NEP' [NEQ' [? ?]]]].
 simpl in H0.
 destruct (eq_dec id id').
-- subst id'. rewrite PTree.gss in H0. inv H0.
+- subst id'. rewrite Maps.PTree.gss in H0. inv H0.
   destruct H2 as [? [? ?]]; subst. unfold fundef in H0; simpl in H0. congruence.
 - exists id', NEP', NEQ'; split; auto.
-  simpl. rewrite PTree.gso in H0 by auto; auto.
+  simpl. rewrite Maps.PTree.gso in H0 by auto; auto.
 Qed.
 
 Definition main_params (ge: genv) start : Prop :=
@@ -763,7 +667,7 @@ assert (exists f, In (id, f) (prog_funct prog)). {
   clear - H1 H0.
   revert G H1 H0; induction g; destruct G; intros; simpl in *.
   exfalso.
-  rewrite PTree.gempty in H1; inv H1.
+  rewrite Maps.PTree.gempty in H1; inv H1.
   inv H0.
   destruct a; simpl in *; subst.
   destruct (eq_dec i id). subst; eauto.
@@ -772,7 +676,7 @@ assert (exists f, In (id, f) (prog_funct prog)). {
   inv H0.
   simpl in H1.
   destruct (ident_eq i0 id). subst. eauto.
-  destruct (IHg G); auto. rewrite PTree.gso in H1; auto.
+  destruct (IHg G); auto. rewrite Maps.PTree.gso in H1; auto.
   eauto.
 }
 destruct H2 as [f ?].
@@ -792,12 +696,12 @@ assert (H9: In (id, mk_funspec f0 cc0 A a a0 P_ne Q_ne) G). {
   clear - H1.
   simpl in H1. unfold make_tycontext_g in H1; simpl in H1.
   induction G; simpl in *.
-  rewrite PTree.gempty in H1; inv H1.
+  rewrite Maps.PTree.gempty in H1; inv H1.
   destruct (ident_eq (fst a1) id); subst.
   destruct a1; simpl in *.
-  rewrite PTree.gss in H1; inv H1. left; auto.
+  rewrite Maps.PTree.gss in H1; inv H1. left; auto.
   destruct a1; simpl in *.
-  rewrite PTree.gso in H1; auto.
+  rewrite Maps.PTree.gso in H1; auto.
 }
 rewrite (find_id_i _ _ _ H9); auto.
 clear - H0 H. unfold prog_defs_names, prog_funct in *.
@@ -871,7 +775,7 @@ forget (prog_funct prog) as g.
 clear - H1 H0.
 revert G H1 H0; induction g; destruct G; intros; simpl in *.
 exfalso.
-rewrite PTree.gempty in H1; inv H1.
+rewrite Maps.PTree.gempty in H1; inv H1.
 inv H0.
 destruct a; simpl in *; subst.
 destruct (eq_dec i id). subst; eauto.
@@ -880,7 +784,7 @@ destruct a. destruct p.
 inv H0.
 simpl in H1.
 destruct (ident_eq i0 id). subst. eauto.
-destruct (IHg G); auto. rewrite PTree.gso in H1; auto.
+destruct (IHg G); auto. rewrite Maps.PTree.gso in H1; auto.
 eauto.
 }
 destruct H2 as [f ?].
@@ -900,12 +804,12 @@ assert (H9: In (id, mk_funspec f0 cc0 A a a0 P_ne Q_ne) G). {
 clear - H1.
 simpl in H1. unfold make_tycontext_g in H1; simpl in H1.
 induction G; simpl in *.
-rewrite PTree.gempty in H1; inv H1.
+rewrite Maps.PTree.gempty in H1; inv H1.
 destruct (ident_eq (fst a1) id); subst.
 destruct a1; simpl in *.
-rewrite PTree.gss in H1; inv H1. left; auto.
+rewrite Maps.PTree.gss in H1; inv H1. left; auto.
 destruct a1; simpl in *.
-rewrite PTree.gso in H1; auto.
+rewrite Maps.PTree.gso in H1; auto.
 }
 rewrite (find_id_i _ _ _ H9); auto.
 clear - H0 H. unfold prog_defs_names, prog_funct in *.
@@ -1123,7 +1027,7 @@ forall id t l vs G,
 list_norepet (map fst l) ->
 match_globvars (prog_vars' l) vs = true ->
 match_fdecs (prog_funct' l) G ->
-((make_tycontext_g vs G) ! id = Some t <->
+((make_tycontext_g vs G) !! id = Some t <->
 ((exists f, In (id,f) G /\ t = type_of_funspec f) \/ In (id,t) vs)).
 Proof.
 intros.
@@ -1160,20 +1064,20 @@ apply iff_trans with (In (id, t) vs );
 [ | clear; intuition; destruct H0 as [? [? ?]]; contradiction].
 revert vs H0; induction vl; destruct vs; simpl in *; intros.
 +(* fl = nil /\ vl = nil /\ vs = nil*)
-rewrite PTree.gempty.
+rewrite Maps.PTree.gempty.
 split; intros. discriminate. contradiction.
 + (* fl = nil /\ vl = nil /\ vs<>nil *)
 clear H2.
 destruct p. inv H0.
 + (* fl = nil /\ vl inductive case /\ vs = nil  *)
-clear H0. rewrite PTree.gempty.
+clear H0. rewrite Maps.PTree.gempty.
 clear. intuition congruence.
 + (* fl = nil /\ vl inductive case /\ vs <> nil *)
 destruct p. destruct a. simpl in *. inv H2.
 specialize (IHvl H4).
 destruct (ident_eq id i).
 - subst id.
-rewrite PTree.gss. split; intro. inv H.
+rewrite Maps.PTree.gss. split; intro. inv H.
 auto.
 destruct H. inv H. auto.
 pose proof (eqb_ident_spec i i0); destruct (eqb_ident i i0).
@@ -1186,7 +1090,7 @@ clear H1.
 pose proof (match_globvars_norepet _ _ H4 H0).
 inv H1. contradiction H7. apply in_map_fst with t; auto.
 - (* id <> i *)
-rewrite PTree.gso by auto.
+rewrite Maps.PTree.gso by auto.
 pose proof (eqb_ident_spec i i0).
 destruct (ident_eq i i0).
 subst. destruct H. rewrite H1 in H0 by auto.
@@ -1197,7 +1101,7 @@ rewrite IHvl; auto.
 clear - n; intuition. inv H0; congruence.
 destruct (eqb_ident i i0). contradict n0; apply H; auto.
 eapply iff_trans; [ | apply (IHvl ((i,t0)::vs))]; clear IHvl.
-simpl;  rewrite PTree.gso by auto. apply iff_refl.
+simpl;  rewrite Maps.PTree.gso by auto. apply iff_refl.
 auto.
 *
 inv H1.
@@ -1205,7 +1109,7 @@ inv H1.
 inv H2.
 specialize (IHfl _ H5 H6).
 destruct (ident_eq id i). subst.
-simpl; rewrite PTree.gss.
+simpl; rewrite Maps.PTree.gss.
 split; intro.
 left; exists fspec.  inv H; auto.
 f_equal.
@@ -1218,7 +1122,7 @@ contradiction H3. apply in_app_iff; right.
 subst.
 eapply match_globvars_in; eauto.
 apply in_map_fst in H; auto.
-simpl; rewrite PTree.gso; auto.
+simpl; rewrite Maps.PTree.gso; auto.
 rewrite IHfl. clear IHfl.
 split; intros [[f [? ?]]| ?]; subst.
 left; eauto. right; eauto.
@@ -1274,7 +1178,7 @@ match_globvars (prog_vars prog) vs = true ->
 match_fdecs (prog_funct prog) G ->
 typecheck_environ
   (Delta1 vs G) (construct_rho (filter_genv (globalenv prog)) empty_env
-    (PTree.set 1 (Vptr b Ptrofs.zero) (PTree.empty val))) .
+    (Maps.PTree.set 1 (Vptr b Ptrofs.zero) (Maps.PTree.empty val))) .
 Proof.
 unfold Delta1; intros.
 unfold construct_rho.
@@ -1290,16 +1194,16 @@ unfold typecheck_temp_environ.
 unfold make_tenv.
 unfold Map.get.
 intros.
-rewrite PTree.gsspec in *. if_tac. inv H2.
+rewrite Maps.PTree.gsspec in *. if_tac. inv H2.
 + exists (Vptr b Ptrofs.zero); split; auto. apply tc_val_tc_val'. simpl; auto.
-+ rewrite PTree.gempty in H2. congruence.
++ rewrite Maps.PTree.gempty in H2. congruence.
 *
 unfold var_types.
 unfold typecheck_var_environ. intros.
 unfold make_tycontext_v. simpl.
-rewrite PTree.gempty.
+rewrite Maps.PTree.gempty.
 unfold Map.get, make_venv, empty_env.
-rewrite PTree.gempty.
+rewrite Maps.PTree.gempty.
 intuition. inv H2. destruct H2; inv H2.
 *
 unfold glob_types. unfold make_tycontext_t, snd.
@@ -1369,11 +1273,11 @@ pose proof initial_mem_core as E.
 unfold juicy_mem_core in *. erewrite E; try reflexivity.
 Qed.
 
-Lemma find_id_maketycontext_s G id : (make_tycontext_s G) ! id = find_id id G.
+Lemma find_id_maketycontext_s G id : (make_tycontext_s G) !! id = find_id id G.
 Proof.
 induction G as [|(i,t) G]; simpl.
 - destruct id; reflexivity.
-- rewrite PTree.gsspec.
+- rewrite Maps.PTree.gsspec.
 do 2 if_tac; congruence.
 Qed.
 
@@ -1385,7 +1289,7 @@ Qed.
 (**************Adaptation of seplog.funspecs_assert, plus lemmas ********)
 (*Maybe this definition can replace seplog.funassert globally?. In fact it
   really needs a genvinron as parameter, not a genviron * list val*)
-Definition funspecs_gassert (FunSpecs: PTree.t funspec): argsassert :=
+Definition funspecs_gassert (FunSpecs: Maps.PTree.t funspec): argsassert :=
  fun gargs => let g := fst gargs in
    (ALL  id: ident, ALL fs:_,  !! (FunSpecs!id = Some fs) -->
               EX b:block,
@@ -1483,7 +1387,7 @@ Qed.
 Lemma believe_cs_ext:
  forall CS Espec Delta ge1 ge2 Delta' n,
   @genv_genv ge1 = @genv_genv ge2 ->
-  PTree.elements (@genv_cenv ge1) = PTree.elements (@genv_cenv ge2) ->
+  Maps.PTree.elements (@genv_cenv ge1) = Maps.PTree.elements (@genv_cenv ge2) ->
   @believe CS Espec Delta ge1 Delta' n ->
   @believe CS Espec Delta ge2 Delta' n.
 Proof.
@@ -1597,9 +1501,9 @@ assert (HGG: cenv_sub (@cenv_cs CS) (globalenv prog)).
  { clear - CSEQ. forget (@cenv_cs CS) as cs1.
    subst psi. forget (genv_cenv (globalenv prog)) as cs2.
    hnf; intros; hnf.
-   destruct (cs1 ! i) eqn:?H; auto.
-   apply PTree.elements_correct in H.
-   apply PTree.elements_complete. congruence.
+   destruct (cs1 !! i) eqn:?H; auto.
+   apply Maps.PTree.elements_correct in H.
+   apply Maps.PTree.elements_complete. congruence.
  }
 
 (***  cut here ****)
@@ -1918,7 +1822,7 @@ assert (H23: app_pred (fungassert Delta (filter_genv psi, args)) (m_phi jm'')).
  simpl. f_equal. unfold eval_id, construct_rho; simpl.
   inv H21.
  erewrite pass_params_ni; try eassumption.
-  rewrite PTree.gss. reflexivity.
+  rewrite Maps.PTree.gss. reflexivity.
  eapply IHfn_params; try eassumption.
 +
  destruct H18 as [H18a [_ H18c]]. subst params.
@@ -2126,9 +2030,9 @@ Proof. induction G1; simpl; intros. right; trivial.
 destruct a. destruct (eq_dec i i0); [ left; trivial | eauto].
 Qed.
 
-Lemma make_tycontext_s_app_inv i fs G1 G2 (G: (make_tycontext_s (G1 ++ G2)) ! i = Some fs):
-  (make_tycontext_s G1) ! i = Some fs \/ (make_tycontext_s G2) ! i = Some fs.
-Proof. rewrite ! find_id_maketycontext_s  in *. apply find_id_app; trivial. Qed.
+Lemma make_tycontext_s_app_inv i fs G1 G2 (G: (make_tycontext_s (G1 ++ G2)) !! i = Some fs):
+  (make_tycontext_s G1) !! i = Some fs \/ (make_tycontext_s G2) !! i = Some fs.
+Proof. rewrite !! find_id_maketycontext_s  in *. apply find_id_app; trivial. Qed.
 
 Lemma believe_app {cs} ge V H G1 G2 n
 (B1: @believe cs Espec (nofunc_tycontext V H) ge (nofunc_tycontext V G1) n)
@@ -2155,7 +2059,7 @@ Qed.
 
 Lemma semax_func_subsumption ge cs V V' F F'
   (SUB: tycontext_sub (nofunc_tycontext V F) (nofunc_tycontext V F'))
-  (HV: forall id, sub_option (make_tycontext_g V F) ! id (make_tycontext_g V' F') ! id):
+  (HV: forall id, sub_option (make_tycontext_g V F) !! id (make_tycontext_g V' F') !! id):
 forall funs G (SF: @semax_func V F cs ge funs G),  @semax_func V' F' cs ge funs G.
 Proof.
 intros. destruct SF as [MF [GC B]]. split; [trivial | split; [ trivial | intros]]. specialize (B _ Gfs Gffp n).
@@ -2163,20 +2067,20 @@ assert (TS: forall f, tycontext_sub (func_tycontext' f (nofunc_tycontext V F)) (
 { clear - SUB HV.
 destruct SUB as [SUBa [SUBb [SUBc [SUBd [SUBe SUBf]]]]]; simpl in *.
 unfold func_tycontext'; split; simpl; intuition.
-destruct ((make_tycontext_t (fn_params f) (fn_temps f)) ! id); trivial. }
+destruct ((make_tycontext_t (fn_params f) (fn_temps f)) !! id); trivial. }
 eapply believe_monoL; [eassumption | apply cspecs_sub_refl | eassumption].
 Qed.
 
 Lemma semax_func_join {cs ge V1 H1 V2 H2 V funs1 funs2 G1 G2 H}
   (SF1: @semax_func V1 H1 cs ge funs1 G1) (SF2: @semax_func V2 H2 cs ge funs2 G2)
 
-  (K1: forall i, sub_option ((make_tycontext_g V1 H1) ! i) ((make_tycontext_g V1 H) ! i))
-  (K2: forall i, subsumespec ((make_tycontext_s H1) ! i) ((make_tycontext_s H) ! i))
-  (K3: forall i, sub_option ((make_tycontext_g V1 H) ! i) ((make_tycontext_g V H) ! i))
+  (K1: forall i, sub_option ((make_tycontext_g V1 H1) !! i) ((make_tycontext_g V1 H) !! i))
+  (K2: forall i, subsumespec ((make_tycontext_s H1) !! i) ((make_tycontext_s H) !! i))
+  (K3: forall i, sub_option ((make_tycontext_g V1 H) !! i) ((make_tycontext_g V H) !! i))
 
-  (N1: forall i, sub_option ((make_tycontext_g V2 H2) ! i) ((make_tycontext_g V2 H) ! i))
-  (N2: forall i, subsumespec ((make_tycontext_s H2) ! i) ((make_tycontext_s H) ! i))
-  (N3: forall i, sub_option ((make_tycontext_g V2 H) ! i) ((make_tycontext_g V H) ! i)):
+  (N1: forall i, sub_option ((make_tycontext_g V2 H2) !! i) ((make_tycontext_g V2 H) !! i))
+  (N2: forall i, subsumespec ((make_tycontext_s H2) !! i) ((make_tycontext_s H) !! i))
+  (N3: forall i, sub_option ((make_tycontext_g V2 H) !! i) ((make_tycontext_g V H) !! i)):
 @semax_func V H cs ge (funs1 ++ funs2) (G1++G2).
 Proof.
 apply semax_func_app.
@@ -2192,11 +2096,11 @@ Qed.
 Lemma semax_func_join_sameV {cs ge H1 H2 V funs1 funs2 G1 G2 H}
   (SF1: @semax_func V H1 cs ge funs1 G1) (SF2: @semax_func V H2 cs ge funs2 G2)
 
-  (K1: forall i, sub_option ((make_tycontext_g V H1) ! i) ((make_tycontext_g V H) ! i))
-  (K2: forall i, subsumespec ((make_tycontext_s H1) ! i) ((make_tycontext_s H) ! i))
+  (K1: forall i, sub_option ((make_tycontext_g V H1) !! i) ((make_tycontext_g V H) !! i))
+  (K2: forall i, subsumespec ((make_tycontext_s H1) !! i) ((make_tycontext_s H) !! i))
 
-  (N1: forall i, sub_option ((make_tycontext_g V H2) ! i) ((make_tycontext_g V H) ! i))
-  (N2: forall i, subsumespec ((make_tycontext_s H2) ! i) ((make_tycontext_s H) ! i)):
+  (N1: forall i, sub_option ((make_tycontext_g V H2) !! i) ((make_tycontext_g V H) !! i))
+  (N2: forall i, subsumespec ((make_tycontext_s H2) !! i) ((make_tycontext_s H) !! i)):
 @semax_func V H cs ge (funs1 ++ funs2) (G1++G2).
 Proof. apply (semax_func_join SF1 SF2); try eassumption; intros; apply sub_option_refl. Qed.
 
@@ -2206,33 +2110,33 @@ destruct x1 as [fs1 |]; destruct x2 as [fs2 |]; trivial; inv H.
 apply subsumespec_refl.
 Qed.
 
-Lemma make_tycontext_g_nilV_elim G i t: (make_tycontext_g nil G) ! i = Some t ->
+Lemma make_tycontext_g_nilV_elim G i t: (make_tycontext_g nil G) !! i = Some t ->
   exists fs, find (fun x => ident_eq i (fst x)) G = Some (i,fs) /\ t=type_of_funspec fs.
 Proof.
-induction G; simpl; intros. rewrite PTree.gempty in H. congruence.
+induction G; simpl; intros. rewrite Maps.PTree.gempty in H. congruence.
 destruct a as [j fs]; unfold ident_eq; simpl in *.
-rewrite PTree.gsspec in H. destruct (peq i j); subst; simpl; eauto.
+rewrite Maps.PTree.gsspec in H. destruct (peq i j); subst; simpl; eauto.
 inv H. exists fs; split; trivial.
 Qed.
 
-Lemma make_tycontext_s_g V H i fs (HH: (make_tycontext_s H) ! i = Some fs):
-  (make_tycontext_g V H) ! i = Some (type_of_funspec fs).
+Lemma make_tycontext_s_g V H i fs (HH: (make_tycontext_s H) !! i = Some fs):
+  (make_tycontext_g V H) !! i = Some (type_of_funspec fs).
 Proof.
-induction H; simpl in *.  rewrite PTree.gempty in HH; congruence.
-destruct a as [j gs]; simpl in *.  rewrite PTree.gsspec.
+induction H; simpl in *.  rewrite Maps.PTree.gempty in HH; congruence.
+destruct a as [j gs]; simpl in *.  rewrite Maps.PTree.gsspec.
 destruct (peq i j); subst.
-+ rewrite PTree.gss in HH; inv HH; trivial.
-+ rewrite PTree.gso in HH; auto.
++ rewrite Maps.PTree.gss in HH; inv HH; trivial.
++ rewrite Maps.PTree.gso in HH; auto.
 Qed.
 
 Lemma make_tycontext_g_consV_elim:
 forall i t v vs G (HV: list_norepet ((map fst (v::vs)) ++ (map fst G))),
-(make_tycontext_g (v::vs) G) ! i = Some t ->
-if peq i (fst v) then t=snd v else (make_tycontext_g vs G) ! i = Some t.
+(make_tycontext_g (v::vs) G) !! i = Some t ->
+if peq i (fst v) then t=snd v else (make_tycontext_g vs G) !! i = Some t.
 Proof.
 intros. destruct v as [j u]. induction G; simpl in *.
-+ rewrite PTree.gsspec in H. destruct (peq i j); subst; trivial. inv H; trivial.
-+ destruct a as [k s]; simpl in *.  rewrite PTree.gsspec in *.
++ rewrite Maps.PTree.gsspec in H. destruct (peq i j); subst; trivial. inv H; trivial.
++ destruct a as [k s]; simpl in *.  rewrite Maps.PTree.gsspec in *.
 destruct (peq i k); subst.
 - inv H. destruct (peq k j); trivial; subst. clear - HV. inv HV.
 elim H1; clear. apply in_or_app.  right; left; trivial.
@@ -2245,12 +2149,12 @@ destruct H2 as [? [? ?]]. constructor.
 Qed.
 Lemma make_tycontext_g_consV_mk:
 forall i t v vs G (HV: list_norepet ((map fst (v::vs)) ++ (map fst G))),
-(if peq i (fst v) then t=snd v else (make_tycontext_g vs G) ! i = Some t) ->
-(make_tycontext_g (v::vs) G) ! i = Some t.
+(if peq i (fst v) then t=snd v else (make_tycontext_g vs G) !! i = Some t) ->
+(make_tycontext_g (v::vs) G) !! i = Some t.
 Proof.
 intros. destruct v as [j u]. simpl in *. induction G; simpl in *. rewrite app_nil_r in HV.
-+ rewrite PTree.gsspec. destruct (peq i j); subst; trivial.
-+ destruct a as [k s]; simpl in *. rewrite PTree.gsspec in *.
++ rewrite Maps.PTree.gsspec. destruct (peq i j); subst; trivial.
++ destruct a as [k s]; simpl in *. rewrite Maps.PTree.gsspec in *.
 destruct (peq i k); subst.
 - destruct (peq k j); trivial; subst. clear - HV. inv HV.
 elim H1; clear. apply in_or_app.  right; left; trivial.
@@ -2262,32 +2166,32 @@ destruct H2 as [? [? ?]]. constructor.
   clear - H2. hnf; intros. apply H2; trivial.  right; trivial.
 Qed.
 
-Lemma make_tycontext_g_nilG_find_id V i: (make_tycontext_g V nil) ! i = find_id i V.
+Lemma make_tycontext_g_nilG_find_id V i: (make_tycontext_g V nil) !! i = find_id i V.
 Proof.
-induction V; simpl. apply PTree.gempty.
+induction V; simpl. apply Maps.PTree.gempty.
 destruct a as [j t]; simpl.
-rewrite PTree.gsspec. unfold eq_dec, EqDec_ident, ident_eq. destruct (peq i j); subst; simpl; eauto.
+rewrite Maps.PTree.gsspec. unfold eq_dec, EqDec_ident, ident_eq. destruct (peq i j); subst; simpl; eauto.
 Qed.
 
-Lemma make_tycontext_g_consG_elim i t V g G (HG: (make_tycontext_g V (g::G)) ! i = Some t):
-if peq i (fst g) then t=type_of_funspec (snd g) else (make_tycontext_g V G) ! i = Some t.
+Lemma make_tycontext_g_consG_elim i t V g G (HG: (make_tycontext_g V (g::G)) !! i = Some t):
+if peq i (fst g) then t=type_of_funspec (snd g) else (make_tycontext_g V G) !! i = Some t.
 Proof.
 destruct g as [j fs]; simpl in *.
-rewrite PTree.gsspec in HG. destruct (peq i j); subst; auto. inv HG; trivial.
+rewrite Maps.PTree.gsspec in HG. destruct (peq i j); subst; auto. inv HG; trivial.
 Qed.
 Lemma make_tycontext_g_consG_mk i t V g G
-  (HG: if peq i (fst g) then t=type_of_funspec (snd g) else (make_tycontext_g V G) ! i = Some t):
-(make_tycontext_g V (g::G)) ! i = Some t.
+  (HG: if peq i (fst g) then t=type_of_funspec (snd g) else (make_tycontext_g V G) !! i = Some t):
+(make_tycontext_g V (g::G)) !! i = Some t.
 Proof.
 destruct g as [j fs]; simpl in *.
-rewrite PTree.gsspec. destruct (peq i j); subst; auto.
+rewrite Maps.PTree.gsspec. destruct (peq i j); subst; auto.
 Qed.
 
 Lemma make_tycontext_g_G_None V i: forall G, find_id i G = None ->
-   (make_tycontext_g V G) ! i = find_id i V.
+   (make_tycontext_g V G) !! i = find_id i V.
 Proof. induction G; intros.
 + apply semax_prog.make_tycontext_g_nilG_find_id.
-+ simpl in H. destruct a as [j a]; simpl. rewrite PTree.gsspec.
++ simpl in H. destruct a as [j a]; simpl. rewrite Maps.PTree.gsspec.
   if_tac in H; subst. inv H. rewrite if_false; auto.
 Qed.
 
@@ -2299,7 +2203,7 @@ intros x y X Y. apply D; [ trivial | right; trivial].
 Qed.
 
 Lemma make_context_g_mk_findV_mk: forall H V (VH:list_norepet (map fst V ++ map fst H)) i t
-(Heqd : find_id i V = Some t), (make_tycontext_g V H) ! i = Some t.
+(Heqd : find_id i V = Some t), (make_tycontext_g V H) !! i = Some t.
 Proof.
 induction H; intros.
 + rewrite make_tycontext_g_nilG_find_id; trivial.
@@ -2313,7 +2217,7 @@ Qed.
 
 Lemma make_context_g_char:
 forall H V (VH:list_norepet (map fst V ++ map fst H)) i,
-(make_tycontext_g V H) ! i = match (make_tycontext_s H)!i with
+(make_tycontext_g V H) !! i = match (make_tycontext_s H)!i with
                                None => find_id i V
                              | Some fs => Some (type_of_funspec fs)
                              end.
@@ -2322,23 +2226,23 @@ induction H; intros.
 + rewrite make_tycontext_g_nilG_find_id.
 simpl. trivial.
 + apply list_norepet_cut_middle in VH.
-remember ((make_tycontext_g V (a :: H)) ! i) as d; symmetry in Heqd; destruct d.
-- apply make_tycontext_g_consG_elim in Heqd. destruct a as [j fs]; simpl in *. rewrite PTree.gsspec.
+remember ((make_tycontext_g V (a :: H)) !! i) as d; symmetry in Heqd; destruct d.
+- apply make_tycontext_g_consG_elim in Heqd. destruct a as [j fs]; simpl in *. rewrite Maps.PTree.gsspec.
 destruct (peq i j); subst; simpl in *; trivial. rewrite <- IHlist, Heqd; trivial.
-- destruct a as [j fs]; simpl in *; rewrite PTree.gsspec in *.
+- destruct a as [j fs]; simpl in *; rewrite Maps.PTree.gsspec in *.
 destruct (peq i j); subst; simpl in *. congruence.
 rewrite <- IHlist, Heqd; trivial.
 Qed.
 
 Lemma suboption_make_tycontext_s_g V G H
-  (GH: forall i : positive, sub_option (make_tycontext_s G) ! i (make_tycontext_s H) ! i)
+  (GH: forall i : positive, sub_option (make_tycontext_s G) !! i (make_tycontext_s H) !! i)
   (VH: list_norepet (map fst V ++ map fst H))
   (LNR : list_norepet (map fst G)) i:
-sub_option (make_tycontext_g V G) ! i (make_tycontext_g V H) ! i.
+sub_option (make_tycontext_g V G) !! i (make_tycontext_g V H) !! i.
 Proof.
-remember ((make_tycontext_g V G) ! i) as d; destruct d; simpl; trivial; symmetry in Heqd.
+remember ((make_tycontext_g V G) !! i) as d; destruct d; simpl; trivial; symmetry in Heqd.
 rewrite make_context_g_char in *; trivial.
-- remember ((make_tycontext_s G) ! i) as q; destruct q.
+- remember ((make_tycontext_s G) !! i) as q; destruct q.
 * specialize (GH i). rewrite <- Heqq in GH; simpl in GH. rewrite GH; trivial.
 * rewrite Heqd, find_id_maketycontext_s. apply find_id_In_map_fst in Heqd.
   remember (find_id i H) as w; destruct w; trivial. symmetry in Heqw; apply find_id_e in Heqw.
@@ -2355,8 +2259,8 @@ Qed.
 Lemma semax_func_join_sameV' {cs ge H1 H2 V funs1 funs2 G1 G2 H}
   (SF1: @semax_func V H1 cs ge funs1 G1) (SF2: @semax_func V H2 cs ge funs2 G2)
 
-  (K1: forall i, sub_option ((make_tycontext_s H1) ! i) ((make_tycontext_s H) ! i))
-  (K2: forall i, sub_option ((make_tycontext_s H2) ! i) ((make_tycontext_s H) ! i))
+  (K1: forall i, sub_option ((make_tycontext_s H1) !! i) ((make_tycontext_s H) !! i))
+  (K2: forall i, sub_option ((make_tycontext_s H2) !! i) ((make_tycontext_s H) !! i))
 
   (LNR: list_norepet ((map fst V)++(map fst H)))
   (LNR1: list_norepet (map fst H1)) (LNR2: list_norepet (map fst H2)):
@@ -2433,7 +2337,7 @@ Lemma semax_external_binaryintersection {ef A1 P1 Q1 P1ne Q1ne A2 P2 Q2 P2ne Q2n
 Proof.
   intros ge ts x.
   simpl in BI.
-  rewrite ! if_true in BI by trivial.
+  rewrite !! if_true in BI by trivial.
   inv BI. apply inj_pair2 in H1; subst P. apply inj_pair2 in H2; subst Q.
   destruct x as [bb BB]; destruct bb.
   * apply (EXT1 ge ts BB).
@@ -2502,7 +2406,7 @@ Proof.
     EX ts1:list Type, EX x1 : dependent_type_functor_rec ts1 A mpred,
     EX FR: mpred,
     !!(forall rho' : environ,
-              !! tc_environ (rettype_tycontext (snd sig)) rho' && (FR * Q ts1 x1 rho') |-- (Q' ts x rho')) &&
+              !! tc_environ (rettype_tycontext (snd sig)) rho' && (FR * Q ts1 x1 rho') ⊢ (Q' ts x rho')) &&
       (stackframe_of f tau * FR * P ts1 x1 (ge_of tau, vals) &&
             !! (map (Map.get (te_of tau)) (map fst (fn_params f)) = map Some vals /\ tc_vals (map snd (fn_params f)) vals))).
  - intros rho m [TC [OM [m1 [m2 [JM [[vals [[MAP VUNDEF] HP']] M2]]]]]].
@@ -2537,7 +2441,7 @@ Proof.
       apply Map.ext; intros x. specialize (Hve x).
       destruct (Map.get ve x); simpl.
       * destruct p; simpl in *. destruct (Hve t) as [_ H]; clear Hve.
-        exploit H. exists b; trivial. rewrite PTree.gempty. congruence.
+        exploit H. exists b; trivial. rewrite Maps.PTree.gempty. congruence.
       * reflexivity.
     + apply join_comm in JA. rewrite sepcon_assoc.
       exists a2, a1; split3; trivial.
@@ -2545,12 +2449,12 @@ Proof.
       clear - MAP VUNDEF TC1 LNR. forget (fn_params f) as params. forget (fn_temps f) as temps. forget (te_of rho) as tau.
       clear f rho. generalize dependent vals. induction params; simpl; intros; destruct vals; inv MAP; trivial.
       inv VUNDEF. inv LNR. destruct a; simpl in *.
-      assert (X: forall id ty, (make_tycontext_t params temps) ! id = Some ty ->
+      assert (X: forall id ty, (make_tycontext_t params temps) !! id = Some ty ->
                  exists v : val, Map.get tau id = Some v /\ tc_val' ty v).
-      { intros. apply TC1. simpl.  rewrite PTree.gso; trivial.
+      { intros. apply TC1. simpl.  rewrite Maps.PTree.gso; trivial.
         apply make_context_t_get in H. intros ?; subst id. contradiction. }
       split; [ clear IHparams | apply (IHparams H6 X _ H1 H4)].
-      destruct (TC1 i t) as [u [U TU]]; clear TC1. rewrite PTree.gss; trivial.
+      destruct (TC1 i t) as [u [U TU]]; clear TC1. rewrite Maps.PTree.gss; trivial.
       rewrite U in H0; inv H0. apply TU; trivial.
  - clear Sub.
    apply extract_exists_pre; intros vals.
@@ -2599,29 +2503,29 @@ Proof.
 Qed.
 
 Lemma make_tycontext_s_distinct : forall a l (Ha : In a l) (Hdistinct : NoDup (map fst l)),
-  (make_tycontext_s l) ! (fst a) = Some (snd a).
+  (make_tycontext_s l) !! (fst a) = Some (snd a).
 Proof.
   intros a l. unfold make_tycontext_s.
   induction l; simpl; intros.
   contradiction.
   inv Hdistinct. destruct a0. simpl in *.
   destruct Ha. subst.
-  simpl. rewrite PTree.gss. auto.
-  rewrite PTree.gso.
+  simpl. rewrite Maps.PTree.gss. auto.
+  rewrite Maps.PTree.gso.
   apply IHl; auto.
   intro; subst.
   apply H1; apply in_map. auto.
 Qed.
 
-(* Maybe the following two lemmas should be put in PTree. *)
+(* Maybe the following two lemmas should be put in Maps.PTree. *)
 
 Lemma lookup_distinct : forall {A B} (f : A -> B) a l t (Ha : In a l) (Hdistinct : NoDup (map fst l)),
-  (fold_right (fun v : ident * A => PTree.set (fst v) (f (snd v))) t l) ! (fst a) =
+  (fold_right (fun v : ident * A => Maps.PTree.set (fst v) (f (snd v))) t l) !! (fst a) =
   Some (f (snd a)).
 Proof.
   induction l; simpl; intros; [contradiction|].
   inv Hdistinct.
-  rewrite PTree.gsspec.
+  rewrite Maps.PTree.gsspec.
   destruct (peq (fst a) (fst a0)) eqn: Heq; setoid_rewrite Heq.
   - destruct Ha; [subst; auto|].
     contradiction H1; rewrite in_map_iff; eauto.
@@ -2631,10 +2535,10 @@ Proof.
 Qed.
 
 Lemma lookup_out : forall {A B} (f : A -> B) a l t (Ha : ~In a (map fst l)),
-  (fold_right (fun v : ident * A => PTree.set (fst v) (f (snd v))) t l) ! a = t ! a.
+  (fold_right (fun v : ident * A => Maps.PTree.set (fst v) (f (snd v))) t l) !! a = t !! a.
 Proof.
   induction l; simpl; intros; auto.
-  rewrite PTree.gsspec.
+  rewrite Maps.PTree.gsspec.
   destruct (peq a (fst a0)) eqn: Heq; setoid_rewrite Heq.
   - contradiction Ha; auto.
   - apply IHl.
@@ -2649,12 +2553,12 @@ Proof.
   unfold func_tycontext, make_tycontext, tycontext_sub; simpl.
   apply sublist.NoDup_app in Hdistinct; destruct Hdistinct as (? & ? & Hdistinct); auto.
   repeat split; auto; intro.
-  - destruct (PTree.get _ _); auto.
+  - destruct (Maps.PTree.get _ _); auto.
   - unfold make_tycontext_g.
     revert dependent G2; revert dependent V2; revert V; induction G; simpl.
     + induction V; simpl; intros. auto.
         rewrite sublist.incl_cons_iff in HV; destruct HV.
-        rewrite PTree.gsspec.
+        rewrite Maps.PTree.gsspec.
         destruct (peq id (fst a)); eauto; subst; simpl.
         rewrite lookup_out.
         apply (lookup_distinct (@id type)); auto.
@@ -2662,7 +2566,7 @@ Proof.
           rewrite in_map_iff; eexists; split; eauto. }
     + intros.
       rewrite sublist.incl_cons_iff in HG; destruct HG.
-      rewrite PTree.gsspec.
+      rewrite Maps.PTree.gsspec.
       destruct (peq id (fst a)); eauto; subst; simpl.
       apply lookup_distinct; auto.
   - unfold make_tycontext_s.
@@ -2670,7 +2574,7 @@ Proof.
     + auto.
     + destruct a; simpl. hnf.
       rewrite sublist.incl_cons_iff in HG; destruct HG.
-      rewrite PTree.gsspec.
+      rewrite Maps.PTree.gsspec.
       fold make_tycontext_s in *.
       destruct (peq id i); eauto; subst; simpl.
       * exists f0; split; [ | apply funspec_sub_si_refl].
