veric/initial_world.v
@@ -1,22 +1,18 @@
-Require Import VST.msl.age_to.
+Require Import VST.zlist.sublist.
 Require Import VST.veric.juicy_base.
 Require Import VST.veric.juicy_mem.
 Require Import VST.veric.juicy_mem_lemmas.
-Require Import VST.veric.juicy_mem_ops.
+(*Require Import VST.veric.juicy_mem_ops.*)
 Require Import VST.veric.res_predicates.
 
 Require Import VST.veric.shares.
 Require Import VST.veric.mpred.
-Require Import VST.veric.age_to_resource_at.
-Import compcert.lib.Maps.
-
-Local Open Scope pred.
 
 Obligation Tactic := idtac.
 
 Lemma adr_range_divide:
   forall b i p q loc,
-    p >= 0 -> q >= 0 -> (adr_range (b,i) (p+q) loc <-> (adr_range (b,i) p loc \/adr_range (b,i+p) q loc)).
+    p >= 0 -> q >= 0 -> (adr_range (b,i) (p+q) loc <-> (adr_range (b,i) p loc \/ adr_range (b,i+p) q loc)).
 Proof.
 split; intros.
 destruct loc as [b' z']; destruct H1.
@@ -25,7 +21,7 @@ destruct H3; [left|right]; split; auto; lia.
 destruct loc as [b' z']; destruct H1; destruct H1; split; auto; lia.
 Qed.
 
-Lemma VALspec_range_e:
+(*Lemma VALspec_range_e:
   forall n sh base m loc, VALspec_range n sh base  m ->
                                 adr_range base n loc -> 
                 {x | m @ loc = YES sh (snd x) (VAL (fst x)) NoneP}.
@@ -42,7 +38,7 @@ simpl.
 destruct H as [? [? ?]]. 
 inv H.
 apply YES_ext; auto.
-Qed.
+Qed.*)
 
 Lemma store_init_data_outside':
   forall F V (ge: Genv.t F V)  b a m p m',
@@ -93,33 +89,19 @@ Proof.
   right. auto.
 Qed.
 
-Ltac destruct_cjoin phi HH :=
-  match goal with
-   |   |- context [@proj1_sig rmap _ ?X] => destruct X as [phi HH]; simpl
-   |  H: context [@proj1_sig rmap _ ?X] |- _ => destruct X as [phi HH]; simpl in H
-  end.
-
 Lemma split_top_neq: fst (Share.split Share.top) <> Share.top.
 Proof.
 case_eq (Share.split Share.top); intros; simpl.
 eapply nonemp_split_neq1; eauto.
 Qed.
 
-Lemma dec_pure: forall r, {exists k, exists pp, r = PURE k pp}+{core r = NO Share.bot bot_unreadable}.
-Proof.
- destruct r.
- right; apply core_NO.
- right; apply core_YES.
- left; eauto.
-Qed.
-
-Lemma store_init_data_list_lem:
+(*Lemma store_init_data_list_lem:
   forall F V (ge: Genv.t F V) m b lo d m',
         Genv.store_init_data_list ge m b lo d = Some m' ->
     forall w IOK IOK' P sh (wsh: writable_share sh),
-     ((P * VALspec_range (init_data_list_size d) sh (b,lo))%pred
+     ((P ∗ VALspec_range (init_data_list_size d) sh (b,lo))%pred
              (m_phi (initial_mem m w IOK))) ->
-     ((P * VALspec_range (init_data_list_size d) sh (b,lo))%pred
+     ((P ∗ VALspec_range (init_data_list_size d) sh (b,lo))%pred
               (m_phi (initial_mem m' w IOK'))).
 Proof.
 intros until 1. intros.
@@ -241,7 +223,7 @@ apply H6.
 do 3 red. rewrite H2.
 rewrite if_false; auto.
 apply core_identity.
-Qed.
+Qed.*)
 
 Lemma fold_right_rev_left:
   forall (A B: Type) (f: A -> B -> A) (l: list B) (i: A),
@@ -323,7 +305,7 @@ Lemma find_id_app2 {A} i x G2: forall G1, list_norepet (map fst (G1++G2)) ->
     rewrite map_app. apply in_or_app; right. apply H0.
   Qed.
 
-Definition initial_core' {F} (ge: Genv.t (fundef F) type) (G: funspecs) (n: nat) (loc: address) : resource :=
+(*Definition initial_core' {F} (ge: Genv.t (fundef F) type) (G: funspecs) (n: nat) (loc: address) : resource :=
    if Z.eq_dec (snd loc) 0
    then match Genv.invert_symbol ge (fst loc) with
            | Some id =>
@@ -508,23 +490,21 @@ Proof.
       resource_at_make_rmap.
     rewrite <- core_resource_at, resource_fmap_core'; auto.
   - unfold wsat_rmap; rewrite ghost_of_make_rmap, !age_to_ghost_of, ghost_of_make_rmap; auto.
-Qed.
+Qed.*)
 
 Lemma list_disjoint_rev2:
    forall A (l1 l2: list A), list_disjoint l1 (rev l2) = list_disjoint l1 l2.
 Proof.
 intros.
 unfold list_disjoint.
-apply prop_ext; split; intros; eapply H; eauto.
+apply Axioms.prop_ext; split; intros; eapply H; eauto.
 rewrite <- In_rev; auto.
 rewrite In_rev; auto.
 Qed.
 
 Require Import VST.veric.mapsto_memory_block.
 
-Open Scope pred.
-
-Lemma writable_blocks_app:
+(*Lemma writable_blocks_app:
   forall bl bl' rho, writable_blocks (bl++bl') rho = writable_blocks bl rho * writable_blocks bl' rho.
 Proof.
 induction bl; intros.
@@ -534,7 +514,7 @@ destruct a as [b n]; simpl.
 rewrite sepcon_assoc.
 f_equal.
 apply IHbl.
-Qed.
+Qed.*)
 
 Fixpoint prog_funct' {F V} (l: list (ident * globdef F V)) : list (ident * F) :=
  match l with nil => nil | (i,Gfun f)::r => (i,f):: prog_funct' r | _::r => prog_funct' r
@@ -550,9 +530,9 @@ Lemma find_symbol_add_globals_nil:
 Proof. intros. simpl.
        unfold Genv.find_symbol, Genv.add_global in *; simpl.
       destruct (eq_dec i id); subst.
-        rewrite PTree.gss. intuition. congruence.
-        rewrite PTree.gso by auto. split; intro Hx.
-        rewrite PTree.gempty in Hx; inv Hx.
+        rewrite Maps.PTree.gss. intuition. congruence.
+        rewrite -> Maps.PTree.gso by auto. split; intro Hx.
+        rewrite Maps.PTree.gempty in Hx; inv Hx.
          inv Hx. congruence.
 Qed.
 
@@ -565,7 +545,7 @@ Lemma find_symbol_add_globals_cons:
 Proof.
 intros.
   assert (Genv.genv_next (Genv.empty_genv F V prog_pub) = 1%positive)  by reflexivity.
-  assert (Genv.find_symbol (Genv.empty_genv F V prog_pub)  id = None) by (intros; apply PTree.gempty).
+  assert (Genv.find_symbol (Genv.empty_genv F V prog_pub)  id = None) by (intros; apply Maps.PTree.gempty).
  forget (Genv.empty_genv F V prog_pub) as ge.
  forget (1%positive) as n.
   revert ge n H H0 H1 H2 HD; induction dl; intros.
@@ -573,7 +553,7 @@ intros.
         simpl in *. rewrite Zlength_nil in HD. lia.
   (*induction step*)
         simpl; auto.
-        rewrite Zlength_cons in *.
+        rewrite -> Zlength_cons in *.
         destruct a as [a ag]; simpl in *.
         destruct dl.
           simpl in *. clear IHdl.
@@ -581,17 +561,17 @@ intros.
           clear H; destruct H3.
           destruct (eq_dec id a).
             subst id. unfold Genv.find_symbol, Genv.add_global; simpl.
-              rewrite PTree.gso; trivial. rewrite H1.
-              rewrite PTree.gss.
+              rewrite Maps.PTree.gso; trivial. rewrite H1.
+              rewrite Maps.PTree.gss.
               split; intro; try congruence. assert (n = n+1)%positive. clear - H4. congruence. lia.
           unfold Genv.find_symbol, Genv.add_global; simpl.
             rewrite H1.
             destruct (eq_dec id i).
               subst i.
-              rewrite PTree.gss. rewrite Pplus_one_succ_r.
+              rewrite Maps.PTree.gss. rewrite Pplus_one_succ_r.
                 split; intro; try congruence. trivial.
-              rewrite PTree.gso; trivial.
-              rewrite PTree.gso; trivial.
+              rewrite Maps.PTree.gso; trivial.
+              rewrite Maps.PTree.gso; trivial.
               unfold Genv.find_symbol in H2. rewrite H2.
               split; intros. congruence. subst. exfalso. apply n1; trivial.
 
@@ -600,8 +580,7 @@ intros.
         2: { clear - n dl. rewrite Z2Pos.inj_succ.
                    rewrite Pplus_one_succ_r. rewrite Pplus_one_succ_l.
                      rewrite Pos.add_assoc. trivial.
-                   rewrite Zlength_correct. simpl.
-                     rewrite Pos.of_nat_succ. apply Pos2Z.is_pos. }
+                   rewrite Zlength_correct. simpl. lia. }
         simpl in H0. inv H0.
         assert (a<>i /\ ~ In i (map fst (p::dl))) by (clear - H; intuition).
         clear H; destruct H0.
@@ -615,7 +594,7 @@ intros.
              simpl in H3. destruct H3; try congruence.
          forget ((p::dl) ++ (i, g) :: nil) as vl.
          assert (Genv.find_symbol (Genv.add_global ge (a,ag)) a = Some (Genv.genv_next ge)).
-            unfold Genv.find_symbol, Genv.add_global; simpl. rewrite PTree.gss; auto.
+            unfold Genv.find_symbol, Genv.add_global; simpl. rewrite Maps.PTree.gss; auto.
 
          forget (Genv.add_global ge (a,ag)) as ge1.
          forget (Genv.genv_next ge) as N; clear ge H2.
@@ -626,14 +605,13 @@ intros.
             inversion2 H1 H4; lia.
          apply (IHvl (Genv.add_global ge1 a0) K H2); auto.
            unfold Genv.find_symbol, Genv.add_global in H4|-*; simpl in *.
-           rewrite PTree.gso; auto.
+           rewrite Maps.PTree.gso; auto.
 
 
          apply IHdl; auto.
         unfold Genv.find_symbol, Genv.add_global in H2|-*; simpl.
-                 rewrite PTree.gso; auto.
-                   rewrite Zlength_correct. simpl.
-                     rewrite Pos.of_nat_succ. apply Pos2Z.is_pos.
+                 rewrite Maps.PTree.gso; auto.
+                   rewrite Zlength_correct. simpl. lia.
 Qed.
 
 Lemma find_symbol_add_globals:
@@ -654,8 +632,7 @@ intros.
 destruct dl.
   intros; apply find_symbol_add_globals_nil.
   apply find_symbol_add_globals_cons; trivial.
-    rewrite Zlength_correct. simpl.
-    rewrite Pos.of_nat_succ. apply Pos2Z.is_pos.
+    rewrite Zlength_correct. simpl. lia.
 Qed.
 
 
@@ -677,22 +654,13 @@ intros.
 destruct dl.
   intros; apply find_symbol_add_globals_nil.
   apply find_symbol_add_globals_cons; trivial.
-    rewrite Zlength_correct. simpl.
-    rewrite Pos.of_nat_succ. apply Pos2Z.is_pos.
+    rewrite Zlength_correct. simpl. lia.
 Qed.
 
 Lemma nth_error_app: forall {T} (al bl : list T) (j: nat),
      nth_error (al++bl) (length al + j) = nth_error bl j.
 Proof.
  intros. induction al; simpl; auto.
-Qed.
-
-Lemma nth_error_app1: forall {T} (al bl : list T) (j: nat),
-     (j < length al)%nat ->
-     nth_error (al++bl) j = nth_error al j.
-Proof.
-  intros. revert al H; induction j; destruct al; simpl; intros; auto; try lia.
-   apply IHj. lia.
 Qed.
 
 Lemma nth_error_rev:
@@ -707,29 +675,15 @@ Proof.
  rewrite <- (Nat.add_0_r (length (rev vl))).
  rewrite nth_error_app.
  case_eq (length vl); intros. simpl. auto.
- replace (S n - n - 1)%nat with O by lia.
+ simpl. replace (S n - n - 1)%nat with O by lia.
  simpl; auto.
- rewrite nth_error_app1 by (rewrite rev_length; lia).
- rewrite IHvl by lia. clear IHvl.
+ rewrite -> nth_error_app1 by (rewrite rev_length; lia).
+ rewrite -> IHvl by lia. clear IHvl.
  destruct n; destruct (length vl). congruence.
  simpl. replace (n-0)%nat with n by lia; auto.
  lia.
- replace (S n1 - n - 1)%nat with (S (S n1 - S n - 1))%nat by lia.
+ simpl; replace (S n1 - n - 1)%nat with (S (S n1 - S n - 1))%nat by lia.
  reflexivity.
-Qed.
-
-Lemma Zlength_app: forall T (al bl: list T),
-    Zlength (al++bl) = Zlength al + Zlength bl.
-Proof. induction al; intros. simpl app; rewrite Zlength_nil; lia.
- simpl app; repeat rewrite Zlength_cons; rewrite IHal; lia.
-Qed.
-Lemma Zlength_rev: forall T (vl: list T), Zlength (rev vl) = Zlength vl.
-Proof. induction vl; simpl; auto. rewrite Zlength_cons. rewrite <- IHvl.
-rewrite Zlength_app. rewrite Zlength_cons. rewrite Zlength_nil; lia.
-Qed.
-
-Lemma Zlength_map: forall A B (f: A -> B) l, Zlength (map f l) = Zlength l.
-Proof. induction l; simpl; auto. repeat rewrite Zlength_cons. f_equal; auto.
 Qed.
 
 (*Partial attempt at porting add_globals_hack*)
@@ -738,7 +692,7 @@ Lemma add_globals_hack_nil {F}:
     gev = Genv.add_globals (Genv.empty_genv (fundef F) type prog_pub) (rev nil) ->
    forall id, Genv.find_symbol gev id = None.
 Proof. simpl; intros; subst.
-  unfold Genv.find_symbol, Genv.empty_genv. simpl. apply PTree.gempty.
+  unfold Genv.find_symbol, Genv.empty_genv. simpl. apply Maps.PTree.gempty.
 Qed.
 
 Lemma add_globals_hack_single {F}:
@@ -748,11 +702,11 @@ Lemma add_globals_hack_single {F}:
 Proof. simpl; intros; subst.
   unfold Genv.find_symbol, Genv.empty_genv. simpl.
   destruct (peq (fst v) id).
-     subst id. rewrite PTree.gss.
+     subst id. rewrite Maps.PTree.gss.
        split; intros. split; trivial. congruence.
        destruct H; subst. trivial.
-  rewrite PTree.gso.
-    split; intros. rewrite PTree.gempty in H. inv H.
+  rewrite Maps.PTree.gso.
+    split; intros. rewrite Maps.PTree.gempty in H. inv H.
     destruct H; subst. congruence.
   auto.
 Qed.
@@ -764,14 +718,13 @@ Proof.
   simpl Pos.of_nat. rewrite Pos.add_comm. symmetry. apply Pos.add_sub.
   simpl length. rewrite IHvl. rewrite Pplus_one_succ_l.
   f_equal.
-  symmetry; rewrite Nat2Pos.inj_succ by lia.
+  symmetry; rewrite -> Nat2Pos.inj_succ by lia.
   rewrite Pplus_one_succ_r. symmetry; apply Pos.add_assoc.
 Qed.
 
 Lemma Zpos_Posofnat: forall n, (n>0)%nat -> Z.pos (Pos.of_nat n) = Z.of_nat n.
 Proof.
- intros. destruct n. lia. simpl  Z.of_nat. f_equal.
- symmetry; apply Pos.of_nat_succ.
+ intros. destruct n. lia. simpl  Z.of_nat. f_equal. lia.
 Qed.
 
 Lemma add_globals_hack {F}:
@@ -799,8 +752,8 @@ Proof. intros. subst.
   rename H1 into Hb; revert H; induction vl; simpl rev; simpl map;
        simpl Genv.find_symbol; intros;
        try rewrite Zlength_nil in *.
-      unfold Genv.find_symbol. rewrite PTree.gempty.
-     intuition.
+      unfold Genv.find_symbol. rewrite Maps.PTree.gempty.
+     intuition; try done. rewrite -> nth_error_nil in *; done.
        destruct a. inv H. rewrite Zlength_cons in Hb.
        destruct (eq_dec (Z.pos b-1) (Zlength vl)).
         clear IHvl Hb. rewrite e. rewrite Zlength_correct.
@@ -833,7 +786,7 @@ Proof. intros. subst.
     unfold Genv.find_symbol, Genv.add_global.
     simpl Genv.genv_symb.
     destruct (eq_dec id i).
-    + subst i. rewrite PTree.gss.
+    + subst i. rewrite Maps.PTree.gss.
       rewrite Genv.genv_next_add_globals.
       rewrite advance_next_length.
       simpl Genv.genv_next.
@@ -844,7 +797,7 @@ Proof. intros. subst.
         clear H; rename H' into H.
           subst b. exfalso; apply n; clear.
           rewrite <- Zlength_rev. rewrite Zlength_correct. forget (length (rev vl)) as i.
-          rewrite Zpos_Posofnat by lia. rewrite Nat2Z.inj_succ. unfold Z.succ.  lia.
+          rewrite -> Zpos_Posofnat by lia. rewrite Nat2Z.inj_succ. unfold Z.succ.  lia.
      - exfalso.
        assert (Z.pos b-1 >= 0) by (clear - Hb; lia).
        pose proof (Z2Nat.id _ (Z.ge_le _ _ H0)).
@@ -859,7 +812,7 @@ Proof. intros. subst.
        revert al H2 H; clear; induction j; destruct al; simpl; intros; auto. inv H; intuition.
        exfalso; clear - H; induction j; inv H; auto.
        f_equal. apply IHj; auto.
-    + rewrite PTree.gso by auto.
+    + rewrite -> Maps.PTree.gso by auto.
       rewrite map_app.
       destruct IHvl.
       split; intro.
@@ -883,7 +836,7 @@ Proof. intros. subst.
           rewrite H0. forget (map fst (rev vl) ++ map fst ((i, g) :: nil)) as al.
           clear - H1. revert al H1; induction j; destruct al; simpl in *; intros; inv H1; auto; try lia.
           specialize (IHj _ H0); lia. }
-        rewrite nth_error_app1 in H1 by auto.
+        rewrite -> nth_error_app1 in H1 by auto.
         apply H0 in H1. auto.
 Qed.
 
@@ -902,20 +855,19 @@ assert (RANGE: 0 <= Z.pos b - 1 < Zlength (rev (prog_defs prog))). {
  rewrite <- (rev_involutive (prog_defs prog)) in H0.
  clear - H0.
  revert H0; induction (rev (prog_defs prog));  simpl Genv.find_symbol; intros.
- unfold Genv.find_symbol in H0. simpl in H0. rewrite PTree.gempty in H0; inv H0.
+ unfold Genv.find_symbol in H0. simpl in H0. rewrite Maps.PTree.gempty in H0; inv H0.
  rewrite Genv.add_globals_app in H0.
  simpl in H0. destruct a.
  destruct (eq_dec i0 i). subst.
  unfold Genv.add_global, Genv.find_symbol in H0. simpl in H0.
- rewrite PTree.gss  in H0. inv H0.
+ rewrite Maps.PTree.gss in H0. inv H0.
  clear.
  split.
  match goal with |- _ <= Z.pos ?A - _ => pose proof (Zgt_pos_0  A); lia end.
  rewrite Zlength_cons.
- induction l. simpl. lia.
+ induction l. rewrite Zlength_nil /=. lia.
  rewrite Zlength_cons.
- Opaque Z.sub. simpl. Transparent Z.sub.
- rewrite Genv.add_globals_app.
+ rewrite /= Genv.add_globals_app.
    simpl Genv.genv_next.
  match goal with |- context [Pos.succ ?J] =>
   forget J as j
@@ -924,7 +876,7 @@ assert (RANGE: 0 <= Z.pos b - 1 < Zlength (rev (prog_defs prog))). {
  replace (Z.pos (Pos.succ j) - 1) with (Z.succ (Z.pos j - 1)). lia.
   unfold Z.succ.  rewrite Pos2Z.inj_succ.  lia.
  unfold Genv.add_global, Genv.find_symbol in IHl, H0. simpl in H0.
- rewrite PTree.gso in H0 by auto.
+ rewrite -> Maps.PTree.gso in H0 by auto.
  apply IHl in H0.
  rewrite Zlength_cons. lia.
  }
@@ -949,9 +901,9 @@ assert (RANGE: 0 <= Z.pos b - 1 < Zlength (rev (prog_defs prog))). {
  clear - RANGE.
  rewrite Zlength_rev in RANGE. rewrite Zlength_correct in RANGE.
  rewrite <- (Z2Nat.id (Z.pos b)) in * by lia.
- rewrite Z2Nat.inj_pos in *.
+ rewrite -> Z2Nat.inj_pos in *.
  forget (Pos.to_nat b) as n. clear b.
- replace (Z.of_nat n - 1) with (Z.of_nat (n-1)) by (rewrite inj_minus1 by lia; f_equal; auto).
+ replace (Z.of_nat n - 1) with (Z.of_nat (n-1)) by (rewrite -> inj_minus1 by lia; f_equal; auto).
  rewrite Nat2Z.id.
  lia.
  inv H1.
@@ -1028,7 +980,7 @@ Proof. intros.
 Qed.
 
 Lemma alloc_globals_rev_nextblock:
-  forall {F V} (ge: Genv.t F V) vl m, alloc_globals_rev ge empty vl = Some m ->
+  forall {F V} (ge: Genv.t F V) vl m, alloc_globals_rev ge Mem.empty vl = Some m ->
      nextblock m = Z.to_pos(Z.succ (Zlength vl)).
 Proof.
   intros.
@@ -1080,7 +1032,7 @@ Proof.
  transitivity (contents_at m' loc).
  Transparent store. unfold store in e0.
  remember (valid_access_dec m Mint8unsigned b p Writable) as d.
- destruct d; inv e0. unfold contents_at; simpl. rewrite PMap.gso by auto. auto.
+ destruct d; inv e0. unfold contents_at; simpl. rewrite -> Maps.PMap.gso by auto. auto.
  eapply IHR_store_zeros; eauto.
  Opaque store.
 Qed.
@@ -1105,7 +1057,7 @@ Proof.
  simpl in *.
  Transparent alloc. unfold alloc in H. Opaque alloc.
  inv H; simpl in *.
- rewrite PMap.gss. repeat rewrite (PMap.gso _ _ NEQ). auto.
+ rewrite Maps.PMap.gss. repeat rewrite (Maps.PMap.gso _ _ NEQ). auto.
 *
  forget (init_data_list_size (gvar_init v)) as N.
  revert H; case_eq (alloc m 0 N); intros.
@@ -1117,11 +1069,11 @@ Proof.
  left. intro. subst b0. apply alloc_result in H. contradiction.
  Transparent alloc. unfold alloc in H. Opaque alloc.
  unfold contents_at. inv H. simpl.
- rewrite PMap.gso by auto. auto.
+ rewrite -> Maps.PMap.gso by auto. auto.
  }
  assert (b0=nextblock m) by (inv H; auto). subst b0.
  unfold max_access_at.
- destruct H2 as [H2a H2b]; rewrite H2a,H2b; clear H H2a H2b.
+ destruct H2 as [H2a H2b]; rewrite H2a H2b; clear H H2a H2b.
  rewrite <- (store_zeros_access _ _ _ _ _ H1).
  apply store_zeros_contents1 with (loc:= (b,ofs)) in H1.
  2: simpl; congruence. rewrite H1; clear H1 m0.
@@ -1134,15 +1086,7 @@ Proof.
  destruct (range_perm_dec m2 (nextblock m) 0 N Cur Freeable); inv H5.
  unfold contents_at, access_at, max_access_at in *;
  simpl in *.
-  repeat rewrite (PMap.gso _ _ NEQ). auto.
-Qed.
-
-Program Definition set_ghost (m : rmap) (g : ghost) (Hg : _) :=
-  proj1_sig (make_rmap (resource_at m) g (level m) _ Hg).
-Next Obligation.
-Proof.
-  intros.
-  extensionality; apply resource_at_approx.
+  repeat rewrite (Maps.PMap.gso _ _ NEQ). auto.
 Qed.
 
 Fixpoint prog_vars' {F V} (l: list (ident * globdef F V)) : list (ident * globvar V) :=
@@ -1151,20 +1095,19 @@ Fixpoint prog_vars' {F V} (l: list (ident * globdef F V)) : list (ident * globva
 
 Definition prog_vars {F} (p: program F) := prog_vars' (prog_defs p).
 
-Definition no_locks phi :=
-  forall addr sh sh' z z' P,
-    phi @ addr <> YES sh sh' (LK z z') P.
+Definition no_locks `{heapGS Σ} : mpred := ∀ addr dq z z' R, ¬ addr ↦{dq} (LK z z' R).
 
-Lemma make_tycontext_s_find_id i G : (make_tycontext_s G) ! i = find_id i G.
+Lemma make_tycontext_s_find_id `{heapGS Σ} i G : (make_tycontext_s G) !! i = find_id i G.
 Proof.
   induction G as [| (j, fs) f IHf]. destruct i; reflexivity.
   simpl.
-  rewrite PTree.gsspec.
+  rewrite /lookup /ptree_lookup in IHf |- *.
+  rewrite Maps.PTree.gsspec.
   rewrite IHf.
   reflexivity.
 Qed.
 
-(* How to relate Gamma to funspecs in memory, once we are outside the
+(*(* How to relate Gamma to funspecs in memory, once we are outside the
    semax proofs?  We define 'matchfunspecs' which will be satisfied by
    the initial memory, and preserved under resource_decay / pures_eq /
    aging. *)
@@ -1241,13 +1184,13 @@ Proof.
   rewrite <-fmap_comp. unfold compose.
   rewrite E.
   reflexivity.
-Qed.
+Qed.*)
 
-Lemma level_initial_core {F} ge G n : level (@initial_core F ge G n) = n.
+(*Lemma level_initial_core {F} ge G n : level (@initial_core F ge G n) = n.
 Proof.
   apply level_make_rmap.
-Qed.
+Qed.*)
 
-(* func_at'': func_at without requiring a proof of non-expansiveness *)
+(*(* func_at'': func_at without requiring a proof of non-expansiveness *)
 Definition func_at'' fsig cc A P Q :=
-  pureat (SomeP (SpecArgsTT A) (packPQ P Q)) (FUN fsig cc).
+  pureat (SomeP (SpecArgsTT A) (packPQ P Q)) (FUN fsig cc).*)
